compiler/wasm/README.md
@@ -1,0 +1,15 @@
+WebAssembly backend for CakeML
+
+[wasmLangScript.sml](wasmLangScript.sml):
+WebAssembly (Wasm) syntax
+
+[wasmScript.sml](wasmScript.sml):
+WASM syntax and semantics
+incomplete and possibly incorrect
+NOT YET TESTED AGAINST THE OFFICIAL WASM SPECIFICATION
+
+[wasmSemScript.sml](wasmSemScript.sml):
+WebAssembly (Wasm) syntax
+
+[wasm_parseScript.sml](wasm_parseScript.sml):
+WASM parser -- supports part of WASM text format
